{
  "@context": {
    "@version": 1.1,
    "skos": "http://www.w3.org/2004/02/skos/core#",
    "xsd": "http://www.w3.org/2001/XMLSchema#",
    "schema": "https://schema.org/",
    "dcat": "http://www.w3.org/ns/dcat#",
    "datacite": "https://selgebali.github.io/datacite4.6-jsonld/enum_lists/descriptionTypes.jsonld#",
    "skos:inScheme": { "@type": "@id" },
    "skos:prefLabel": { "@container": "@language" },
    "skos:definition": { "@container": "@language" },
    "skos:notation": { "@type": "xsd:string" }
  },
  "@graph": [
    {
      "@id": "datacite:DescriptionTypeScheme",
      "@type": "skos:ConceptScheme",
      "skos:prefLabel": { "en": "DataCite Description Type" },
      "skos:definition": { "en": "Controlled list of description types as defined in the DataCite Metadata Schema 4.6." }
    },
    {
      "@id": "datacite:Abstract",
      "@type": "skos:Concept",
      "skos:prefLabel": { "en": "Abstract" },
      "skos:definition": { "en": "A brief description of the resource and the context in which the resource was created." },
      "skos:notation": "Abstract",
      "skos:inScheme": "datacite:DescriptionTypeScheme"
    },
    {
      "@id": "datacite:Methods",
      "@type": "skos:Concept",
      "skos:prefLabel": { "en": "Methods" },
      "skos:definition": { "en": "The methodology employed for the study or research." },
      "skos:notation": "Methods",
      "skos:inScheme": "datacite:DescriptionTypeScheme"
    },
    {
      "@id": "datacite:SeriesInformation",
      "@type": "skos:Concept",
      "skos:prefLabel": { "en": "SeriesInformation" },
      "skos:definition": { "en": "Information about a repeating series, such as volume, issue, number." },
      "skos:notation": "SeriesInformation",
      "skos:inScheme": "datacite:DescriptionTypeScheme"
    },
    {
      "@id": "datacite:TableOfContents",
      "@type": "skos:Concept",
      "skos:prefLabel": { "en": "TableOfContents" },
      "skos:definition": { "en": "A listing of the Table of Contents." },
      "skos:notation": "TableOfContents",
      "skos:inScheme": "datacite:DescriptionTypeScheme"
    },
    {
      "@id": "datacite:TechnicalInfo",
      "@type": "skos:Concept",
      "skos:prefLabel": { "en": "TechnicalInfo" },
      "skos:definition": { "en": "Detailed information that may be associated with design, implementation, operation, use, and/or maintenance of a process, system, or instrument." },
      "skos:notation": "TechnicalInfo",
      "skos:inScheme": "datacite:DescriptionTypeScheme"
    },
    {
      "@id": "datacite:Other",
      "@type": "skos:Concept",
      "skos:prefLabel": { "en": "Other" },
      "skos:definition": { "en": "Other description information that does not fit into an existing category." },
      "skos:notation": "Other",
      "skos:inScheme": "datacite:DescriptionTypeScheme"
    }
  ]
}