{
  "@context": {
    "@version": 1.1,
    "skos": "http://www.w3.org/2004/02/skos/core#",
    "xsd": "http://www.w3.org/2001/XMLSchema#",
    "schema": "http://schema.org/",
    "dcat": "http://www.w3.org/ns/dcat#",
    "datacite": "https://selgebali.github.io/datacite4.6-jsonld/enum_lists/relatedIdTypes.jsonld#"
  },
  "@graph": [
    {
      "@id": "datacite:RelatedIdentifierTypeScheme",
      "@type": "skos:ConceptScheme",
      "skos:prefLabel": "Related Identifier Type",
      "skos:definition": "Controlled list of identifier types that can be used in DataCite metadata to relate the described resource to another resource."
    },
    {
      "@id": "datacite:ARK",
      "@type": "skos:Concept",
      "skos:prefLabel": "ARK",
      "skos:definition": "Archival Resource Key, a persistent identifier scheme for information objects of any type.",
      "skos:inScheme": "datacite:RelatedIdentifierTypeScheme",
      "skos:note": "Listed in DataCite controlled list."
    },
    {
      "@id": "datacite:arXiv",
      "@type": "skos:Concept",
      "skos:prefLabel": "arXiv",
      "skos:definition": "Identifier for preprints deposited in the arXiv repository (e.g., arXiv:1501.00001).",
      "skos:inScheme": "datacite:RelatedIdentifierTypeScheme",
      "skos:note": "Listed in DataCite controlled list."
    },
    {
      "@id": "datacite:bibcode",
      "@type": "skos:Concept",
      "skos:prefLabel": "bibcode",
      "skos:definition": "Astrophysics Data System (ADS) bibliographic code, commonly used in astronomy and astrophysics literature.",
      "skos:inScheme": "datacite:RelatedIdentifierTypeScheme",
      "skos:note": "Listed in DataCite controlled list."
    },
    {
      "@id": "datacite:CSTR",
      "@type": "skos:Concept",
      "skos:prefLabel": "CSTR",
      "skos:definition": "Chinese Science and Technology Resource identifier, used for persistent identification in Chinese infrastructures.",
      "skos:inScheme": "datacite:RelatedIdentifierTypeScheme",
      "skos:note": "Added in DataCite 4.4."
    },
    {
      "@id": "datacite:DOI",
      "@type": "skos:Concept",
      "skos:prefLabel": "DOI",
      "skos:definition": "Digital Object Identifier, the primary persistent identifier system used in scholarly communications.",
      "skos:inScheme": "datacite:RelatedIdentifierTypeScheme",
      "skos:note": "Recommended where available."
    },
    {
      "@id": "datacite:EAN13",
      "@type": "skos:Concept",
      "skos:prefLabel": "EAN13",
      "skos:definition": "International Article Number (formerly European Article Number), 13-digit identifier used for barcodes.",
      "skos:inScheme": "datacite:RelatedIdentifierTypeScheme",
      "skos:note": "Listed in DataCite controlled list."
    },
    {
      "@id": "datacite:EISSN",
      "@type": "skos:Concept",
      "skos:prefLabel": "EISSN",
      "skos:definition": "Electronic International Standard Serial Number identifying electronic serials.",
      "skos:inScheme": "datacite:RelatedIdentifierTypeScheme",
      "skos:note": "Listed in DataCite controlled list."
    },
    {
      "@id": "datacite:Handle",
      "@type": "skos:Concept",
      "skos:prefLabel": "Handle",
      "skos:definition": "Handle System identifier for digital objects, of which DOIs are a specific implementation.",
      "skos:inScheme": "datacite:RelatedIdentifierTypeScheme",
      "skos:note": "Listed in DataCite controlled list."
    },
    {
      "@id": "datacite:IGSN",
      "@type": "skos:Concept",
      "skos:prefLabel": "IGSN",
      "skos:definition": "International Generic Sample Number, a persistent identifier for physical samples.",
      "skos:inScheme": "datacite:RelatedIdentifierTypeScheme",
      "skos:note": "Listed in DataCite controlled list."
    },
    {
      "@id": "datacite:ISBN",
      "@type": "skos:Concept",
      "skos:prefLabel": "ISBN",
      "skos:definition": "International Standard Book Number, a unique identifier for books.",
      "skos:inScheme": "datacite:RelatedIdentifierTypeScheme",
      "skos:note": "Listed in DataCite controlled list."
    },
    {
      "@id": "datacite:ISSN",
      "@type": "skos:Concept",
      "skos:prefLabel": "ISSN",
      "skos:definition": "International Standard Serial Number, a unique identifier for serial publications.",
      "skos:inScheme": "datacite:RelatedIdentifierTypeScheme",
      "skos:note": "Listed in DataCite controlled list."
    },
    {
      "@id": "datacite:ISTC",
      "@type": "skos:Concept",
      "skos:prefLabel": "ISTC",
      "skos:definition": "International Standard Text Code, a unique identifier for textual works.",
      "skos:inScheme": "datacite:RelatedIdentifierTypeScheme",
      "skos:note": "Listed in DataCite controlled list."
    },
    {
      "@id": "datacite:LISSN",
      "@type": "skos:Concept",
      "skos:prefLabel": "LISSN",
      "skos:definition": "Linking International Standard Serial Number, used to link different media versions of a continuing resource.",
      "skos:inScheme": "datacite:RelatedIdentifierTypeScheme",
      "skos:note": "Added in DataCite 4.4."
    },
    {
      "@id": "datacite:LSID",
      "@type": "skos:Concept",
      "skos:prefLabel": "LSID",
      "skos:definition": "Life Science Identifier, a persistent identifier for biological objects.",
      "skos:inScheme": "datacite:RelatedIdentifierTypeScheme",
      "skos:note": "Listed in DataCite controlled list."
    },
    {
      "@id": "datacite:PMID",
      "@type": "skos:Concept",
      "skos:prefLabel": "PMID",
      "skos:definition": "PubMed Identifier, a unique number assigned to each PubMed record.",
      "skos:inScheme": "datacite:RelatedIdentifierTypeScheme",
      "skos:note": "Listed in DataCite controlled list."
    },
    {
      "@id": "datacite:PURL",
      "@type": "skos:Concept",
      "skos:prefLabel": "PURL",
      "skos:definition": "Persistent Uniform Resource Locator, a type of URL intended to provide long-lasting references to digital objects.",
      "skos:inScheme": "datacite:RelatedIdentifierTypeScheme",
      "skos:note": "Listed in DataCite controlled list."
    },
    {
      "@id": "datacite:RRID",
      "@type": "skos:Concept",
      "skos:prefLabel": "RRID",
      "skos:definition": "Research Resource Identifier, used to cite key resources such as model organisms, antibodies, and software tools.",
      "skos:inScheme": "datacite:RelatedIdentifierTypeScheme",
      "skos:note": "Added in DataCite 4.1."
    },
    {
      "@id": "datacite:UPC",
      "@type": "skos:Concept",
      "skos:prefLabel": "UPC",
      "skos:definition": "Universal Product Code, widely used identifier for products, especially in retail.",
      "skos:inScheme": "datacite:RelatedIdentifierTypeScheme",
      "skos:note": "Listed in DataCite controlled list."
    },
    {
      "@id": "datacite:URL",
      "@type": "skos:Concept",
      "skos:prefLabel": "URL",
      "skos:definition": "Uniform Resource Locator, a web address identifying a resource on the internet.",
      "skos:inScheme": "datacite:RelatedIdentifierTypeScheme",
      "skos:note": "Listed in DataCite controlled list."
    },
    {
      "@id": "datacite:URN",
      "@type": "skos:Concept",
      "skos:prefLabel": "URN",
      "skos:definition": "Uniform Resource Name, a persistent, location-independent identifier assigned within defined namespaces.",
      "skos:inScheme": "datacite:RelatedIdentifierTypeScheme",
      "skos:note": "Listed in DataCite controlled list."
    },
    {
      "@id": "datacite:w3id",
      "@type": "skos:Concept",
      "skos:prefLabel": "w3id",
      "skos:definition": "Permanent identifier system for web resources under w3id.org, often used for vocabularies and ontologies.",
      "skos:inScheme": "datacite:RelatedIdentifierTypeScheme",
      "skos:note": "Added in DataCite 4.5."
    }
  ]
}
