{
  "@context": {
    "@version": 1.1,
    "skos": "http://www.w3.org/2004/02/skos/core#",
    "xsd": "http://www.w3.org/2001/XMLSchema#",
    "schema": "http://schema.org/",
    "dcat": "http://www.w3.org/ns/dcat#",
    "datacite": "https://selgebali.github.io/datacite4.6-jsonld/titleTypes.jsonld#"
  },
  "@graph": [
    {
      "@id": "datacite:TitleTypeScheme",
      "@type": "skos:ConceptScheme",
      "skos:prefLabel": "Title Type",
      "skos:definition": "Controlled list of title types as defined in the DataCite Metadata Schema (4.6)."
    },
    {
      "@id": "datacite:AlternativeTitle",
      "@type": "skos:Concept",
      "skos:prefLabel": "AlternativeTitle",
      "skos:definition": "Any form of the title used as a substitute or alternative to the main title of the resource.",
      "skos:inScheme": "datacite:TitleTypeScheme",
      "skos:note": "Examples include translated titles or titles commonly used as an alternative name."
    },
    {
      "@id": "datacite:Subtitle",
      "@type": "skos:Concept",
      "skos:prefLabel": "Subtitle",
      "skos:definition": "A secondary title that amplifies or explains the main title.",
      "skos:inScheme": "datacite:TitleTypeScheme",
      "skos:note": "Often clarifies or provides additional context to the main title."
    },
    {
      "@id": "datacite:TranslatedTitle",
      "@type": "skos:Concept",
      "skos:prefLabel": "TranslatedTitle",
      "skos:definition": "The title of the resource translated into another language.",
      "skos:inScheme": "datacite:TitleTypeScheme",
      "skos:note": "The attribute xml:lang is recommended to indicate the language of the translation."
    },
    {
      "@id": "datacite:Other",
      "@type": "skos:Concept",
      "skos:prefLabel": "Other",
      "skos:definition": "A title type that does not fall into AlternativeTitle, Subtitle, or TranslatedTitle.",
      "skos:inScheme": "datacite:TitleTypeScheme",
      "skos:note": "Use only when no other titleType value is appropriate."
    }
  ]
}